Started on server loop. Thought I could get away with a really big recv buffer, but recv hangs until it reads all of its bytes. TODO : write more in the style of recv_ACK, which dynamically receives messages

.Makefile.d
@@ -13,9 +13,9 @@ theories/Monads.vos theories/Monads.vok theories/Monads.required_vos: theories/M
 theories/Messages.vo theories/Messages.glob theories/Messages.v.beautified theories/Messages.required_vo: theories/Messages.v theories/OCamlTypes.vo theories/StringTheory.vo theories/Monads.vo
 theories/Messages.vio: theories/Messages.v theories/OCamlTypes.vio theories/StringTheory.vio theories/Monads.vio
 theories/Messages.vos theories/Messages.vok theories/Messages.required_vos: theories/Messages.v theories/OCamlTypes.vos theories/StringTheory.vos theories/Monads.vos
-theories/Client.vo theories/Client.glob theories/Client.v.beautified theories/Client.required_vo: theories/Client.v theories/Messages.vo theories/Monads.vo
-theories/Client.vio: theories/Client.v theories/Messages.vio theories/Monads.vio
-theories/Client.vos theories/Client.vok theories/Client.required_vos: theories/Client.v theories/Messages.vos theories/Monads.vos
+theories/Client.vo theories/Client.glob theories/Client.v.beautified theories/Client.required_vo: theories/Client.v theories/Messages.vo theories/Monads.vo theories/OCamlTypes.vo
+theories/Client.vio: theories/Client.v theories/Messages.vio theories/Monads.vio theories/OCamlTypes.vio
+theories/Client.vos theories/Client.vok theories/Client.required_vos: theories/Client.v theories/Messages.vos theories/Monads.vos theories/OCamlTypes.vos
 theories/Server.vo theories/Server.glob theories/Server.v.beautified theories/Server.required_vo: theories/Server.v theories/Messages.vo theories/Monads.vo
 theories/Server.vio: theories/Server.v theories/Messages.vio theories/Monads.vio
 theories/Server.vos theories/Server.vok theories/Server.required_vos: theories/Server.v theories/Messages.vos theories/Monads.vos
