proofchat/bin/server/main.ml
@@ -1,6 +1,7 @@
 open Server
+open Proofchat.Logging
 
 let () = print_endline "Hello, World!";
   match server "127.0.0.1" 8888 with
-  | NoneE err -> failwith err
+  | NoneE err -> fatal rc_Error err
   | _ -> ()
