proofchat/lib/logging.ml
@@ -1,0 +1,97 @@
+(** logging.ml - Custom logging and error messages *)
+
+(*
+  The two key functions here are _log and fatal, which do what they sound like
+*)
+
+(** Represents the severity of a log statement *)
+type log_type =
+  | Log_None
+  | Log_Debug
+  | Log_Info
+  | Log_Warning
+  | Log_Error
+  | Log_Critical
+
+let _GLOBAL_LOG_LEVEL = Log_Info
+
+(** Follows the order in the type definition, \[0:5\]*)
+let int_of_log = function
+  | Log_Debug ->
+      1
+  | Log_Info ->
+      2
+  | Log_Warning ->
+      3
+  | Log_Error ->
+      4
+  | Log_Critical ->
+      5
+  | Log_None ->
+      0
+
+(** For exits, their appropriate return code and the message type *)
+type return_code = int * string
+
+let rc_Ok = (0, "OK")
+
+and rc_Error = (1, "ERROR")
+
+(** ANSI encoding for bold text *)
+let ansi_bold = "\x1b[1m"
+
+(** ANSI encoding for red text *)
+let ansi_red = "\x1b[38:5:196m"
+
+(** ANSI encoding for orange text *)
+let ansi_orange = "\x1b[38:5:208m"
+
+(** ANSI encoding for yellow text *)
+let ansi_yellow = "\x1b[38:5:178m"
+
+(** ANSI encoding for plain text *)
+let ansi_reset = "\x1b[0m"
+
+(** ANSI encoding for bold red text *)
+let error_red = ansi_bold ^ ansi_red
+
+(** ANSI encoding for bold orange text *)
+let error_orange = ansi_bold ^ ansi_orange
+
+(** ANSI encoding for bold yellow text *)
+let error_yellow = ansi_bold ^ ansi_yellow
+
+(** Gets the string representation of a {!log_type}*)
+let string_of_log = function
+  | Log_Debug ->
+      ansi_bold ^ "[DEBUG]"
+  | Log_Info ->
+      ansi_bold ^ "[INFO]"
+  | Log_Warning ->
+      ansi_yellow ^ "[WARNING]"
+  | Log_Error ->
+      ansi_orange ^ "[ERROR]"
+  | Log_Critical ->
+      ansi_red ^ "[CRITICAL]"
+  | Log_None ->
+      ansi_reset ^ "[NONE]"
+
+(** A fatal log statement that immediately exits the program *)
+let fatal rc message =
+  Printf.fprintf stderr
+    "%s[%s] - %s%s\n----------------------------------------\n" error_red
+    (snd rc) ansi_reset message ;
+  flush stderr ;
+  exit (fst rc)
+
+(** Prints log statements to stdout/stderr *)
+let _log log_level message =
+  if log_level = Log_None || int_of_log _GLOBAL_LOG_LEVEL > int_of_log log_level
+  then ()
+  else
+    let stream =
+      if log_level = Log_Debug || log_level = Log_Info then stdout else stderr
+    in
+    Printf.fprintf stream "LOG:%s%s - %s\n" (string_of_log log_level) ansi_reset
+      message ;
+    flush stream
